Clean/Gadgets/Rotation64/Theorems.lean
@@ -1,0 +1,16 @@
+import Clean.Types.U64
+import Clean.Utils.Field
+
+variable {p : ℕ} [Fact p.Prime]
+variable [p_large_enough: Fact (p > 512)]
+
+namespace Gadgets.Rotation64.Theorems
+
+def rot64 (x : ℕ) (offset : ℕ) : ℕ :=
+  let offset := offset % 64
+  let low := x % (2^offset)
+  let high := x / (2^offset)
+  low * (2^(64 - offset)) + high
+
+
+end Gadgets.Rotation64.Theorems
